Lean2Js/Builder.lean
@@ -90,6 +90,8 @@ def indexOf (s needle : Expr) : Expr := .strBin .indexOf s needle
 
 def join (xs sep : Expr) : Expr := .strBin .join xs sep
 
+def «repeat» (s n : Expr) : Expr := .strBin .repeat s n
+
 def endsWith (s suffix : Expr) : Expr := .strBin .endsWith s suffix
 def includes (s needle : Expr) : Expr := .strBin .includes s needle
 def split (s sep : Expr) : Expr := .strBin .split s sep
